theories/Logic/Semantics.v
@@ -36,46 +36,46 @@ Section Shallow.
   Local Open Scope ctl_scope.
 
   (*| Binary shallow strong/weak forall [next] modality |*)
-  Definition cax (p q: MP) (t: MS) (w: World E): Prop :=
+  Definition anc (p q: MP) (t: MS) (w: World E): Prop :=
     p t w /\
       can_step t w /\
       (forall t' w', [t,w] ↦ [t', w'] -> q t' w').
   
-  Definition cex(p q: MP) (t: MS) (w: World E): Prop :=
+  Definition enc(p q: MP) (t: MS) (w: World E): Prop :=
     p t w /\
       exists t' w', [t, w] ↦ [t', w'] /\ q t' w'.
-  Hint Unfold cax cex: core.
+  Hint Unfold anc enc: core.
 
   Unset Elimination Schemes.
   (* Forall strong until *)
-  Inductive cau (p q: MP): MP :=
+  Inductive auc (p q: MP): MP :=
   | MatchA: forall t w,       
       q t w ->    (* Matches [q] now; done *)
-      cau p q t w
+      auc p q t w
   | StepA:  forall t w,
-      cax p (cau p q) t w -> (* Matches [p] now; steps to [m'] *)
-      cau p q t w.
+      anc p (auc p q) t w -> (* Matches [p] now; steps to [m'] *)
+      auc p q t w.
 
   (* Exists strong until *)
-  Inductive ceu(p q: MP): MP :=
+  Inductive euc(p q: MP): MP :=
   | MatchE: forall t w,
       q t w ->    (* Matches [q] now; done *)
-      ceu p q t w
+      euc p q t w
   | StepE: forall t w,
-      cex p (ceu p q) t w -> (* Matches [p] now; steps to [m'] *)
-      ceu p q t w.
+      enc p (euc p q) t w -> (* Matches [p] now; steps to [m'] *)
+      euc p q t w.
 
-  (* Custom induction schemes for [cau, ceu] *)
-  Definition cau_ind :
+  (* Custom induction schemes for [auc, euc] *)
+  Definition auc_ind :
     forall [p q: MP] (P : MP),
       (forall t w, q t w -> P t w) -> (* base *)
       (forall t w, (* step *)
-          cax p (cau p q) t w ->
-          cax p P t w ->
+          anc p (auc p q) t w ->
+          anc p P t w ->
          P t w) ->
-      forall t w, cau p q t w -> P t w :=
+      forall t w, auc p q t w -> P t w :=
     fun p q P Hbase Hstep =>
-      fix F (t : MS) (w: World E) (c : cau p q t w) {struct c}: P t w :=
+      fix F (t : MS) (w: World E) (c : auc p q t w) {struct c}: P t w :=
       match c with
       | MatchA _ _ t w y => Hbase t w y
       | @StepA _ _ t w (conj Hp (conj Hs HtrP)) =>
@@ -84,18 +84,18 @@ Section Shallow.
             (conj Hp (conj Hs (fun t' w' tr => F t' w' (HtrP t' w' tr))))
       end.
 
-  Definition ceu_ind :
+  Definition euc_ind :
     forall [p q: MP] (P : MP),
       (forall t w, q t w -> P t w) -> (* base *)
       (forall t w, (* step *)
           p t w /\
             (exists t' w', [t, w] ↦ [t', w']
-                      /\ ceu p q t' w'
+                      /\ euc p q t' w'
                       /\ P t' w') ->
           P t w) ->
-      forall t w, ceu p q t w -> P t w :=
+      forall t w, euc p q t w -> P t w :=
     fun p q P Hbase Hstep =>
-      fix F (t : MS) (w: World E) (c : ceu p q t w) {struct c}: P t w :=
+      fix F (t : MS) (w: World E) (c : euc p q t w) {struct c}: P t w :=
       match c with
       | MatchE _ _ t w y => Hbase t w y
       | @StepE _ _ t w (conj Hp (ex_intro _ t' (ex_intro _ w' (conj tr h)))) =>
@@ -113,14 +113,14 @@ Section Shallow.
   Arguments impl /.  
   (* Always globally *)
   (* Matches [p] now; all paths step to (t', s') *)
-  Program Definition cagF p: mon MP :=
-    {| body := cax p |}.
+  Program Definition agcF p: mon MP :=
+    {| body := anc p |}.
   Next Obligation.
     repeat red; intros; destruct H0; split; destruct H1; auto.
   Qed.
   
-  Program Definition cegF p: mon MP :=
-    {| body := cex p |}.
+  Program Definition egcF p: mon MP :=
+    {| body := enc p |}.
   Next Obligation.
     repeat red; intros; destruct H0 as [H0 (t' & w' & TR & Hx)]; split; auto.
     exists t', w'; auto.
@@ -129,17 +129,17 @@ Section Shallow.
 End Shallow.
 
 (* Companion notations *)
-Notation cag p := (gfp (cagF p)).
-Notation ceg p := (gfp (cegF p)).
-Notation cagt p  := (t (cagF p)).
-Notation cegt p  := (t (cegF p)).
-Notation cagbt p := (bt (cagF p)).
-Notation cegbt p := (bt (cegF p)).
-Notation cagT p  := (T (cagF p)).
-Notation cegT p  := (T (cegF p)).
-Notation cagbT p := (bT (cagF p)).
-Notation cegbT p := (bT (cegF p)).
-#[global] Hint Constructors ceu cau: ctl.
+Notation agc p := (gfp (agcF p)).
+Notation egc p := (gfp (egcF p)).
+Notation agct p  := (t (agcF p)).
+Notation egct p  := (t (egcF p)).
+Notation agcbt p := (bt (agcF p)).
+Notation egcbt p := (bt (egcF p)).
+Notation agcT p  := (T (agcF p)).
+Notation egcT p  := (T (egcF p)).
+Notation agcbT p := (bT (agcF p)).
+Notation egcbT p := (bT (egcF p)).
+#[global] Hint Constructors euc auc: ctl.
 
 (*| Semantics of ctl entailment |*)
 Section Entailment.
@@ -151,12 +151,12 @@ Section Entailment.
     fix entailsL (φ: ctll E): MP X :=
       match φ with
       | (CNow φ) => fun _ w => φ w /\ not_done w
-      | (CuL Q_A p q) => cau (entailsL p) (entailsL q)
-      | (CuL Q_E p q) => ceu (entailsL p) (entailsL q)
-      | (CxL Q_A p q) => cax (entailsL p) (entailsL q)
-      | (CxL Q_E p q) => cex (entailsL p) (entailsL q)
-      | (Cg Q_A φ) => cag (entailsL φ)
-      | (Cg Q_E φ) => ceg (entailsL φ)
+      | (CuL Q_A p q) => auc (entailsL p) (entailsL q)
+      | (CuL Q_E p q) => euc (entailsL p) (entailsL q)
+      | (CxL Q_A p q) => anc (entailsL p) (entailsL q)
+      | (CxL Q_E p q) => enc (entailsL p) (entailsL q)
+      | (Cg Q_A φ) => agc (entailsL φ)
+      | (Cg Q_E φ) => egc (entailsL φ)
       | (CAndL p q) => fun t w => entailsL p t w /\ entailsL q t w
       | (COrL p q) => fun t w => entailsL p t w \/ entailsL q t w
       end.
@@ -165,10 +165,10 @@ Section Entailment.
     fix entailsR (φ: ctlr E X): MP X :=
       match φ with
       | (CDone φ) => fun _ => done_with φ
-      | (CuR Q_A p q) => cau (entailsL X p) (entailsR q)
-      | (CuR Q_E p q) => ceu (entailsL X p) (entailsR q)
-      | (CxR Q_A p q) => cax (entailsL X p) (entailsR q)
-      | (CxR Q_E p q) => cex (entailsL X p) (entailsR q)
+      | (CuR Q_A p q) => auc (entailsL X p) (entailsR q)
+      | (CuR Q_E p q) => euc (entailsL X p) (entailsR q)
+      | (CxR Q_A p q) => anc (entailsL X p) (entailsR q)
+      | (CxR Q_E p q) => enc (entailsL X p) (entailsR q)
       | (CAndR p q) => fun t w => entailsR p t w /\ entailsR q t w
       | (COrR p q) => fun t w => entailsR p t w \/ entailsR q t w
       | (CImplR p q) => fun t w => entailsL X p t w -> entailsR q t w
@@ -177,12 +177,12 @@ Section Entailment.
   Lemma unfold_entailsL {X}: forall (t: M E HE X) (w: World E) (φ: ctll E),
       entailsL X φ t w = match φ with
                          | (CNow φ) => φ w /\ not_done w
-                         | (CuL Q_A p q) => cau (entailsL X p) (entailsL X q) t w
-                         | (CuL Q_E p q) => ceu (entailsL X p) (entailsL X q) t w
-                         | (CxL Q_A p q) => cax (entailsL X p) (entailsL X q) t w
-                         | (CxL Q_E p q) => cex (entailsL X p) (entailsL X q) t w
-                         | (Cg Q_A φ) => cag (entailsL X φ) t w
-                         | (Cg Q_E φ) => ceg (entailsL X φ) t w
+                         | (CuL Q_A p q) => auc (entailsL X p) (entailsL X q) t w
+                         | (CuL Q_E p q) => euc (entailsL X p) (entailsL X q) t w
+                         | (CxL Q_A p q) => anc (entailsL X p) (entailsL X q) t w
+                         | (CxL Q_E p q) => enc (entailsL X p) (entailsL X q) t w
+                         | (Cg Q_A φ) => agc (entailsL X φ) t w
+                         | (Cg Q_E φ) => egc (entailsL X φ) t w
                          | (CAndL p q) => entailsL X p t w /\ entailsL X q t w
                          | (COrL p q) => entailsL X p t w \/ entailsL X q t w
                          end.
@@ -191,10 +191,10 @@ Section Entailment.
   Lemma unfold_entailsR {X}: forall (t: M E HE X) (w: World E) (φ: ctlr E X),
       entailsR φ t w = match φ with
                        | (CDone φ) => done_with φ w
-                       | (CuR Q_A p q) => cau (entailsL X p) (entailsR q) t w
-                       | (CuR Q_E p q) => ceu (entailsL X p) (entailsR q) t w
-                       | (CxR Q_A p q) => cax (entailsL X p) (entailsR q) t w
-                       | (CxR Q_E p q) => cex (entailsL X p) (entailsR q) t w
+                       | (CuR Q_A p q) => auc (entailsL X p) (entailsR q) t w
+                       | (CuR Q_E p q) => euc (entailsL X p) (entailsR q) t w
+                       | (CxR Q_A p q) => anc (entailsL X p) (entailsR q) t w
+                       | (CxR Q_E p q) => enc (entailsL X p) (entailsR q) t w
                        | (CAndR p q) => entailsR p t w /\ entailsR q t w
                        | (COrR p q) => entailsR p t w \/ entailsR q t w
                        | (CImplR p q) => entailsL X p t w -> entailsR q t w
@@ -264,26 +264,26 @@ Lemma ctlr_finish `{KMS: Kripke M E} X:
 Proof. intros; auto. Qed. 
 Global Hint Resolve ctlr_finish: ctlr.
 
-(*| AX, WX, EX unfold |*)
+(*| AN, WX, EN unfold |*)
 Lemma ctll_ax `{KMS: Kripke M E} X:
   forall (t: M E HE X) (w: World E) (p q: ctll E),
-    <( t, w |= p AX q )> <-> <( t, w |= p)> /\ can_step t w /\ forall t' w', [t, w] ↦ [t',w'] -> <( t',w' |= q )>.
+    <( t, w |= p AN q )> <-> <( t, w |= p)> /\ can_step t w /\ forall t' w', [t, w] ↦ [t',w'] -> <( t',w' |= q )>.
 Proof. intros; auto. Qed.
 
 Lemma ctll_ex `{KMS: Kripke M E} X:
   forall (t: M E HE X) (w: World E) (p q: ctll E),
-    <( t,w |= p EX q )> <-> <( t, w|= p)> /\ exists t' w', [t,w] ↦ [t',w'] /\ <( t',w' |= q )>.
+    <( t,w |= p EN q )> <-> <( t, w|= p)> /\ exists t' w', [t,w] ↦ [t',w'] /\ <( t',w' |= q )>.
 Proof. intros; auto. Qed.
 Global Hint Resolve ctll_ax ctll_ex: ctl.
 
 Lemma ctlr_ax `{KMS: Kripke M E} X:
   forall (t: M E HE X) (w: World E) (p: ctll E) (q: ctlr E X),
-    <[ t, w |= p AX q ]> <-> <( t, w |= p)> /\ can_step t w /\ forall t' w', [t, w] ↦ [t',w'] -> <[ t',w' |= q ]>.
+    <[ t, w |= p AN q ]> <-> <( t, w |= p)> /\ can_step t w /\ forall t' w', [t, w] ↦ [t',w'] -> <[ t',w' |= q ]>.
 Proof. intros; auto. Qed.
 
 Lemma ctlr_ex `{KMS: Kripke M E} X:
   forall (t: M E HE X) (w: World E) (p: ctll E) (q: ctlr E X),
-    <[ t,w |= p EX q ]> <-> <( t, w |= p )> /\ exists t' w', [t,w] ↦ [t',w'] /\ <[ t',w' |= q ]>.
+    <[ t,w |= p EN q ]> <-> <( t, w |= p )> /\ exists t' w', [t,w] ↦ [t',w'] /\ <[ t',w' |= q ]>.
 Proof. intros; eauto. Qed.
 Global Hint Resolve ctlr_ax ctlr_ex: ctl.
 
@@ -313,10 +313,10 @@ Lemma ctlr_impll  `{KMS: Kripke M E} X:
     <[ t, w |= p -> q ]> <-> <( t, w |= p )> -> <[ t, w |= q ]>.
 Proof. intros t w p q; rewrite unfold_entailsR; intros [H H']; auto. Qed. 
 
-(* [AX φ] is stronger than [EX φ] *)
+(* [AN φ] is stronger than [EN φ] *)
 Lemma ctll_ax_ex `{KMS: Kripke M E} X:
   forall (t: M E HE X) (w: World E) (p q: ctll E),
-    <( t, w |= p AX q )> -> <( t, w |= p EX q )>.
+    <( t, w |= p AN q )> -> <( t, w |= p EN q )>.
 Proof.
   intros.
   rewrite ctll_ax, ctll_ex in *.
@@ -341,7 +341,7 @@ Qed.
 
 Lemma ctlr_ax_ex `{KMS: Kripke M E} X:
   forall (t: M E HE X) (w: World E) (p: ctll E) (q: ctlr E X),
-    <[ t, w |= p AX q ]> -> <[ t, w |= p EX q ]>.
+    <[ t, w |= p AN q ]> -> <[ t, w |= p EN q ]>.
 Proof.
   intros.
   rewrite ctlr_ax, ctlr_ex in *.
@@ -437,8 +437,8 @@ Proof.
   contradiction.
 Qed.
 
-Lemma cax_not_done `{KMS: Kripke M E} X: forall (t: M E HE X) (w: World E) p q,
-    cax p q t w ->
+Lemma anc_not_done `{KMS: Kripke M E} X: forall (t: M E HE X) (w: World E) p q,
+    anc p q t w ->
     not_done w.
 Proof.
   intros.
@@ -446,15 +446,15 @@ Proof.
   now apply can_step_not_done with t.
 Qed.
 
-Lemma cex_not_done `{KMS: Kripke M E} X: forall (t: M E HE X) (w: World E) p q,
-    cex p q t w ->
+Lemma enc_not_done `{KMS: Kripke M E} X: forall (t: M E HE X) (w: World E) p q,
+    enc p q t w ->
     not_done w.
 Proof.
   intros.
   destruct H as (? & ? & ? & ? & ?).
   now apply ktrans_not_done with t x x0.
 Qed.
-Hint Resolve cex_not_done cax_not_done: ctl.
+Hint Resolve enc_not_done anc_not_done: ctl.
 
 (* Here the syntax separation becomes semantically apparent *)
 Lemma ctll_not_done `{KMS: Kripke M E} X: forall (t: M E HE X) (w: World E) (p: ctll E),
@@ -465,9 +465,9 @@ Proof.
   hinduction p before X; intros;
     rewrite unfold_entailsL in H; eauto; try destruct q; try solve [ destruct H; eauto].
   - destruct H; eauto.
-    now apply cax_not_done in H. 
+    now apply anc_not_done in H. 
   - destruct H; eauto.
-    now apply cex_not_done in H.
+    now apply enc_not_done in H.
   - step in H; destruct H, H0.
     now apply can_step_not_done with t.
   - step in H; destruct H, H0 as (t' & w' & TR & ?).
@@ -534,8 +534,8 @@ Qed.
   let R' := fresh R in
   first [rewrite unfold_entailsL | setoid_rewrite unfold_entailsL];
   coinduction R' CIH;
-  try change (cag (entailsL ?X ?p) ?t ?w) with <( t, w |= AG p )> in *;
-  try change (ceg (entailsL ?X ?p) ?t ?w) with <( t, w |= EG p )> in *.
+  try change (agc (entailsL ?X ?p) ?t ?w) with <( t, w |= AG p )> in *;
+  try change (egc (entailsL ?X ?p) ?t ?w) with <( t, w |= EG p )> in *.
 
 #[global] Tactic Notation "coinduction" simple_intropattern(R) simple_intropattern(H) :=
   (coinduction_g R H || coinduction R H).
